theories/Syntax/StrictPos.v
@@ -4,28 +4,71 @@ Import ListNotations.
 
 Set Default Proof Using "Type".
 
-(* Finitary strictly-positive inductive signatures.
+(* Finitary strictly-positive inductive signatures for indexed inductive families.
 
-   We represent each inductive by a finite list of constructors. Each constructor
-   has a finite list of *non-recursive* parameter types (in some type universe
-   `Ty`) and a finite number of recursive fields.
+   This supports CIC-style indexed inductive types (e.g., Vec A n, Eq A x y, Fin n).
+   
+   An inductive signature consists of:
+   - Uniform parameters (e.g., A in Vec A n)
+   - Indices (e.g., n in Vec A n; x and y in Eq A x y)
+   - A universe level
+   - A list of constructors
 
-   This representation is meant to be consumed by a typing judgement parameterized
-   over a global environment of such signatures.
+   Each constructor has:
+   - Non-recursive argument types
+   - Recursive argument specifications: for each rec field, the list of indices
+     at which that recursive occurrence happens
+   - Result indices: the indices at which this constructor produces a value
+     (e.g., vnil : Vec A 0 has result index [0]; vcons : Vec A n -> Vec A (S n) 
+      has result index [S n])
+
+   This representation is consumed by a typing judgement parameterized over
+   a global environment of such signatures.
 *)
 
 Record ctor_sig (Ty : Type) : Type := {
-  ctor_param_tys : list Ty;
-  ctor_rec_arity : nat;
+  ctor_param_tys : list Ty;        (* non-recursive arguments *)
+  ctor_rec_args : list (list Ty);  (* for each rec field: indices at that occurrence *)
+  ctor_indices : list Ty           (* constructor result indices *)
 }.
+
+Arguments ctor_param_tys {_} _.
+Arguments ctor_rec_args {_} _.
+Arguments ctor_indices {_} _.
 
 Record ind_sig (Ty : Type) : Type := {
-  ind_level : nat;
-  ind_ctors : list (ctor_sig Ty);
+  ind_params : list Ty;            (* uniform parameters *)
+  ind_indices : list Ty;           (* index types (may depend on params) *)
+  ind_level : nat;                 (* universe level *)
+  ind_ctors : list (ctor_sig Ty)   (* constructors *)
 }.
 
+Arguments ind_params {_} _.
+Arguments ind_indices {_} _.
+Arguments ind_level {_} _.
+Arguments ind_ctors {_} _.
+
+(* Helper functions for arities *)
+
 Definition ctor_param_arity {Ty : Type} (c : ctor_sig Ty) : nat :=
-  length (@ctor_param_tys _ c).
+  length (ctor_param_tys c).
+
+Definition ctor_rec_arity {Ty : Type} (c : ctor_sig Ty) : nat :=
+  length (ctor_rec_args c).
+
+Definition ctor_arity {Ty : Type} (c : ctor_sig Ty) : nat :=
+  ctor_param_arity c + ctor_rec_arity c.
+
+Definition ind_param_arity {Ty : Type} (Σ : ind_sig Ty) : nat :=
+  length (ind_params Σ).
+
+Definition ind_index_arity {Ty : Type} (Σ : ind_sig Ty) : nat :=
+  length (ind_indices Σ).
+
+Definition ind_arity {Ty : Type} (Σ : ind_sig Ty) : nat :=
+  ind_param_arity Σ + ind_index_arity Σ.
+
+(* Lookup functions *)
 
 Definition lookup {A : Type} (xs : list A) (n : nat) : option A :=
   nth_error xs n.
@@ -34,10 +77,10 @@ Definition lookup_ind {Ty : Type} (Σenv : list (ind_sig Ty)) (I : nat) : option
   lookup Σenv I.
 
 Definition lookup_ctor {Ty : Type} (Σ : ind_sig Ty) (c : nat) : option (ctor_sig Ty) :=
-  lookup (@ind_ctors _ Σ) c.
+  lookup (ind_ctors Σ) c.
 
 Lemma lookup_ctor_lt {Ty : Type} (Σ : ind_sig Ty) (c : nat) (ctor : ctor_sig Ty) :
-  lookup_ctor Σ c = Some ctor -> c < length (@ind_ctors _ Σ).
+  lookup_ctor Σ c = Some ctor -> c < length (ind_ctors Σ).
 Proof.
   unfold lookup_ctor, lookup.
   intro H.
